Phi_Examples/Dyn_Arr_arbi.thy
@@ -28,7 +28,7 @@ proc len_dynarr:
   input    \<open>l \<Ztypecolon> DynArr addr TY T\<heavy_comma> addr \<Ztypecolon> \<v>\<a>\<l> \<Pp>\<t>\<r> \<d>\<y>\<n>\<a>\<r>\<r>\<close>
   output   \<open>l \<Ztypecolon> DynArr addr TY T\<heavy_comma> length l \<Ztypecolon> \<v>\<a>\<l> \<nat>\<close>
 \<medium_left_bracket>
-  to \<open>OPEN _ _\<close> \<semicolon>
+  \<t>\<r>\<a>\<n>\<s>\<f>\<o>\<r>\<m>\<s>_\<t>\<o> \<o>\<p>\<e>\<n> \<semicolon>
   $addr \<tribullet> len !
   \<open>MAKE _ (DynArr addr _ _)\<close>
 \<medium_right_bracket> .
@@ -47,9 +47,9 @@ proc get_dynarr:
   premises \<open>i < length l\<close>
   output   \<open>l \<Ztypecolon> DynArr addr TY T\<heavy_comma> l!i \<Ztypecolon> \<v>\<a>\<l> T\<close>
 \<medium_left_bracket>
-  to \<open>OPEN _ _\<close> \<semicolon>
+  \<t>\<r>\<a>\<n>\<s>\<f>\<o>\<r>\<m>\<s>_\<t>\<o> \<o>\<p>\<e>\<n> \<semicolon>
   $addr \<tribullet> data ! \<tribullet> $i !
-  \<open>MAKE _ (DynArr addr _ _)\<close>
+  \<m>\<a>\<k>\<e>\<s> \<open>DynArr addr _ _\<close>
 \<medium_right_bracket> .
 
 
@@ -58,9 +58,9 @@ proc set_dynarr:
   premises \<open>i < length l\<close>
   output   \<open>l[i := v] \<Ztypecolon> DynArr addr TY T\<close>
 \<medium_left_bracket>
-  to \<open>OPEN _ _\<close> \<semicolon>
-  $addr \<tribullet> data ! \<tribullet> $i := $v \<semicolon>
- \<open>l[i := v] \<Ztypecolon> MAKE _ (DynArr addr _ _)\<close>
+  \<t>\<r>\<a>\<n>\<s>\<f>\<o>\<r>\<m>\<s>_\<t>\<o> \<o>\<p>\<e>\<n> \<semicolon>
+  $addr \<tribullet> data ! \<tribullet> $i := $v \<semicolon> 
+  \<m>\<a>\<k>\<e>\<s> \<open>l[i := v] \<Ztypecolon> (DynArr addr _ _)\<close>
 \<medium_right_bracket> .
 
 proc Max:
@@ -75,7 +75,7 @@ proc push_dynarr:
   input    \<open>l \<Ztypecolon> DynArr addr TY T\<heavy_comma> addr \<Ztypecolon> \<v>\<a>\<l> \<Pp>\<t>\<r> \<d>\<y>\<n>\<a>\<r>\<r>\<heavy_comma> v \<Ztypecolon> \<v>\<a>\<l> T\<close>
   output   \<open>l @ [v] \<Ztypecolon> DynArr addr TY T\<close>
 \<medium_left_bracket>
-  to \<open>OPEN _ _\<close> \<semicolon>
+  \<t>\<r>\<a>\<n>\<s>\<f>\<o>\<r>\<m>\<s>_\<t>\<o> \<o>\<p>\<e>\<n> \<semicolon>
   val len \<leftarrow> $addr \<tribullet> len ! \<semicolon>
   val cap \<leftarrow> $addr \<tribullet> cap ! \<semicolon>
   if ($cap = $len) \<medium_left_bracket>
@@ -87,11 +87,11 @@ proc push_dynarr:
       $addr \<tribullet> len := $addr \<tribullet> len ! + 1 \<semicolon>
       $addr \<tribullet> cap := $cap' \<semicolon>
       $data' \<tribullet> $len := $v \<semicolon>
-      \<open>l@[v] \<Ztypecolon> MAKE _ (DynArr addr _ _)\<close>
+      \<m>\<a>\<k>\<e>\<s> \<open>l@[v] \<Ztypecolon> DynArr addr _ _\<close>
   \<medium_right_bracket> \<medium_left_bracket>
       $addr \<tribullet> data ! \<tribullet> $len := $v \<semicolon>
       $addr \<tribullet> len := $len + 1 \<semicolon>
-      \<open>l@[v] \<Ztypecolon> MAKE _ (DynArr addr _ _)\<close>
+      \<m>\<a>\<k>\<e>\<s> \<open>l@[v] \<Ztypecolon> DynArr addr _ _\<close>
   \<medium_right_bracket>
 \<medium_right_bracket> .
 
@@ -103,9 +103,9 @@ proc concat_dynarr:
   val len \<leftarrow> len_dynarr ($addr2) \<semicolon>
   replicate_a (\<open>0 \<Ztypecolon> \<nat>\<close>, $len)
               \<open>\<lambda>i. l1 @ take i l2 \<Ztypecolon> DynArr addr1 TY T\<close>
-  \<medium_left_bracket> \<rightarrow> val i ;;
+  \<medium_left_bracket> \<rightarrow> val i \<semicolon>
     push_dynarr ($addr1, get_dynarr ($addr2, $i))
-  \<medium_right_bracket> ;;
+  \<medium_right_bracket>
 \<medium_right_bracket> .
 
 
@@ -117,7 +117,7 @@ proc pop_dynarr:
   premises \<open>l \<noteq> []\<close>
   output   \<open>butlast l \<Ztypecolon> DynArr addr TY T\<heavy_comma> last l \<Ztypecolon> \<v>\<a>\<l> T\<close>
 \<medium_left_bracket>
-  to \<open>OPEN _ _\<close> \<semicolon>
+  \<t>\<r>\<a>\<n>\<s>\<f>\<o>\<r>\<m>\<s>_\<t>\<o> \<o>\<p>\<e>\<n> \<semicolon>
   val len \<leftarrow> $addr \<tribullet> len ! - 1 \<semicolon>
   val half_cap \<leftarrow> ($addr \<tribullet> cap !) / 2 \<semicolon>
   val ret \<leftarrow> $addr \<tribullet> data ! \<tribullet> $len ! \<semicolon>
@@ -128,9 +128,9 @@ proc pop_dynarr:
     mfree ($addr \<tribullet> data !) \<semicolon>
     $addr \<tribullet> data := $data' \<semicolon>
     $addr \<tribullet> cap := $half_cap \<semicolon>
-    \<open>MAKE _ (DynArr addr _ _)\<close>
+    \<m>\<a>\<k>\<e>\<s> \<open>DynArr addr _ _\<close>
   \<medium_right_bracket>
-  \<medium_left_bracket> \<open>MAKE _ (DynArr addr _ _)\<close> \<medium_right_bracket>
+  \<medium_left_bracket> \<m>\<a>\<k>\<e>\<s> \<open>DynArr addr _ _\<close> \<medium_right_bracket>
   $ret
 \<medium_right_bracket> .
 
@@ -141,7 +141,7 @@ proc new_dynarr:
 \<medium_left_bracket>
   val ret \<leftarrow> calloc_1 \<open>\<lbrace> data: \<Pp>\<t>\<r> \<a>\<r>\<r>\<a>\<y>[0] TY, len: \<nat>, cap: \<nat> \<rbrace>\<close> \<semicolon>
   $ret \<tribullet> data := (calloc_aN (\<open>0 \<Ztypecolon> \<nat>\<close>) \<open>T\<close>) \<semicolon>
-  \<open>MAKE _ (DynArr addr _ _)\<close> \<semicolon>
+  \<m>\<a>\<k>\<e>\<s> \<open>DynArr addr _ _\<close> \<semicolon>
   $ret
 \<medium_right_bracket> .
 
@@ -150,7 +150,7 @@ proc del_dynarr:
   input  \<open>l \<Ztypecolon> DynArr addr TY T\<heavy_comma> addr \<Ztypecolon> \<v>\<a>\<l> \<Pp>\<t>\<r> \<d>\<y>\<n>\<a>\<r>\<r>\<close>
   output \<open>Void\<close>
 \<medium_left_bracket>
-  to \<open>OPEN _ _\<close> \<semicolon>
+  \<t>\<r>\<a>\<n>\<s>\<f>\<o>\<r>\<m>\<s>_\<t>\<o> \<o>\<p>\<e>\<n> \<semicolon>
   mfree ($addr \<tribullet> data !) \<semicolon>
   mfree ($addr)
 \<medium_right_bracket> .
@@ -160,11 +160,12 @@ proc map_dynarr:
   requires C: \<open>\<And>x u. \<p>\<r>\<o>\<c> C u \<lbrace> x \<Ztypecolon> \<v>\<a>\<l>[u] T \<longmapsto> f x \<Ztypecolon> \<v>\<a>\<l> T \<rbrace> \<close>
   output \<open>map f l \<Ztypecolon> DynArr addr TY T\<close>
 \<medium_left_bracket>
-  note [\<phi>sledgehammer_simps] = list_eq_iff_nth_eq nth_append ;;
+  note [\<phi>sledgehammer_simps] = list_eq_iff_nth_eq nth_append \<semicolon>
+
   replicate_a (\<open>0 \<Ztypecolon> \<nat>\<close>, len_dynarr ($addr)) \<open>\<lambda>i. (map f (take i l) @ drop i l) \<Ztypecolon> DynArr addr TY T\<close>
-  \<medium_left_bracket> \<rightarrow> val i ;;
+  \<medium_left_bracket> \<rightarrow> val i \<semicolon>
      set_dynarr ($addr, $i, C (get_dynarr ($addr, $i)))
-  \<medium_right_bracket> ;;
+  \<medium_right_bracket>
 \<medium_right_bracket> .
 
 proc exists_dynarr:
@@ -173,10 +174,11 @@ proc exists_dynarr:
   output \<open>l \<Ztypecolon> DynArr addr TY T\<heavy_comma> list_ex P l \<Ztypecolon> \<v>\<a>\<l> \<bool>\<close>
 \<medium_left_bracket>
   var zz \<leftarrow> False ;;
-  replicate_a (\<open>0 \<Ztypecolon> \<nat>\<close>, len_dynarr ($addr))  \<open>\<lambda>i. l \<Ztypecolon> DynArr addr TY T\<heavy_comma> list_ex P (take i l) \<Ztypecolon> \<v>\<a>\<r>[zz] \<bool>\<close> ;;
-    \<medium_left_bracket> \<rightarrow> val i ;;
+  replicate_a (\<open>0 \<Ztypecolon> \<nat>\<close>, len_dynarr ($addr))
+              \<open>\<lambda>i. l \<Ztypecolon> DynArr addr TY T\<heavy_comma> list_ex P (take i l) \<Ztypecolon> \<v>\<a>\<r>[zz] \<bool>\<close> \<semicolon>
+    \<medium_left_bracket> \<rightarrow> val i \<semicolon>
       $zz \<or> C (get_dynarr ($addr, $i)) \<rightarrow> $zz
-    \<medium_right_bracket> ;;
+    \<medium_right_bracket> \<semicolon>
   $zz
 \<medium_right_bracket> .
 
@@ -187,14 +189,14 @@ proc fold_map_dynarr:
        and C: \<open>\<And>x z u v. \<p>\<r>\<o>\<c> C u v \<lbrace> x \<Ztypecolon> \<v>\<a>\<l>[u] T\<heavy_comma> z \<Ztypecolon> \<v>\<a>\<l>[v] U \<longmapsto> f x \<Ztypecolon> \<v>\<a>\<l> T\<heavy_comma> g x z \<Ztypecolon> \<v>\<a>\<l> U \<rbrace> \<close>
   output \<open>map f l \<Ztypecolon> DynArr addr TY T\<heavy_comma> fold g l z0 \<Ztypecolon> \<v>\<a>\<l> U\<close>
 \<medium_left_bracket>
-  var zz \<leftarrow> $z0 ;;
+  var zz \<leftarrow> $z0 \<semicolon>
   replicate_a (\<open>0 \<Ztypecolon> \<nat>\<close>, len_dynarr ($addr))
                \<open>\<lambda>i. (map f (take i l) @ drop i l) \<Ztypecolon> DynArr addr TY T\<heavy_comma> fold g (take i l) z0 \<Ztypecolon> \<v>\<a>\<r>[zz] U\<close>
-  \<medium_left_bracket> \<rightarrow> val i ;;
-    C (get_dynarr ($addr, $i), $zz) \<rightarrow> val x', var zz ;;
+  \<medium_left_bracket> \<rightarrow> val i \<semicolon>
+    C (get_dynarr ($addr, $i), $zz) \<rightarrow> val x', var zz \<semicolon>
     set_dynarr ($addr, $i, $x')
   \<medium_right_bracket> certified by (auto simp add: list_eq_iff_nth_eq nth_append, auto_sledgehammer,
-                  insert \<open>i < length l\<close>, induct i, auto simp add: take_Suc_conv_app_nth) ;;
+                  insert \<open>i < length l\<close>, induct i, auto simp add: take_Suc_conv_app_nth) \<semicolon>
   $zz
 \<medium_right_bracket> .
 
